golf

Incremental/Shake/Standard.lean
@@ -26,8 +26,6 @@ variable [BEq ℭ.Q] [Hashable ℭ.Q]
 @[specialize bracket]
 def fetch
     (bracket : ∀ {α}, ℭ.Q → m α → m α)
-    (bracket_canReturn : ∀ {α} (q : ℭ.Q) (x : m α) (a : α),
-      MonadAttach.CanReturn (bracket q x) a → MonadAttach.CanReturn x a)
     (ι₀ : ∀ i, ℭ.V i) (q₀ : ℭ.Q) :
     StateT (Store hI hR tasks ι₀) m (Value tasks ι₀ q₀) := do
   let (vcache, cache) ← get
@@ -35,7 +33,7 @@ def fetch
   let fetchWithHash (q' : ℭ.Q) (_ : ℭ.rel q' q₀) :
       StateT (Store hI hR tasks ι₀) m
         { vh : Value tasks ι₀ q' × H // vh.snd = (hR q') vh.fst.val } := do
-    let v ← fetch bracket bracket_canReturn ι₀ q'
+    let v ← fetch bracket ι₀ q'
     let (vc, _) ← get
     match vc.get? q' with
     | some e => pure ⟨(v, e.val.snd), by
@@ -43,7 +41,7 @@ def fetch
         exact congrArg (hR q') (e.val.fst.spec.trans v.spec.symm)⟩
     | none => pure ⟨(v, hR q' v.val), rfl⟩
   let doRun : StateT (Store hI hR tasks ι₀) m (Value tasks ι₀ q₀) := do
-    let ⟨(memo, value), _⟩ ← run hI hR tasks ι₀ q₀ bracket bracket_canReturn fetchWithHash
+    let ⟨(memo, value), _⟩ ← run hI hR tasks ι₀ q₀ bracket fetchWithHash
     modify fun (vc, c) =>
       (vc.insert q₀ ⟨(value, hR q₀ value.val), rfl⟩, c.insert q₀ memo)
     pure value
@@ -51,7 +49,7 @@ def fetch
   | some mm =>
     if hvin : verifyInputs hI ι₀ mm.inputDeps then do
       match ← verifyDeps hI hR tasks ι₀
-          (fun q' _hq => fetch bracket bracket_canReturn ι₀ q') mm.queryDeps with
+          (fun q' _hq => fetch bracket ι₀ q') mm.queryDeps with
       | some ⟨hdep⟩ =>
         let value : Value tasks ι₀ q₀ := ⟨mm.value, mm.invariant ι₀
           ((verifyInputs_spec hI ι₀ mm.inputDeps).mp hvin) hdep⟩
@@ -75,10 +73,7 @@ public def Shake
     {H : Type} [DecidableEq H]
     (hI : ∀ i, ℭ.V i ↪ H) (hR : ∀ q, ℭ.R q ↪ H) (tasks : Tasks ℭ)
     {m : Type → Type} [Monad m] [LawfulMonad m] [MonadAttach m] [LawfulMonadAttach m]
-    (bracket : ∀ {α}, ℭ.Q → m α → m α := fun _ x => x)
-    (bracket_canReturn : ∀ {α} (q : ℭ.Q) (x : m α) (a : α),
-      MonadAttach.CanReturn (bracket q x) a → MonadAttach.CanReturn x a :=
-      by intros; assumption) :
+    (bracket : ∀ {α}, ℭ.Q → m α → m α := fun _ x => x) :
     Build ℭ J tasks m Id where
   σ := J × Shake.Cache hI hR tasks
   init j := (j, DHashMap.emptyWithCapacity 1024)
@@ -90,7 +85,7 @@ public def Shake
     let initStore : Shake.Store hI hR tasks ι₀ :=
       (DHashMap.emptyWithCapacity 1024, oldCache)
     let (v, (_, newCache)) ←
-      bracket q (Shake.fetch hI hR tasks bracket bracket_canReturn ι₀ q initStore)
+      bracket q (Shake.fetch (m := m) hI hR tasks bracket ι₀ q initStore)
     pure (v, (j, newCache))
 
 end Incremental
